Intermediate/Typing.lean
@@ -99,9 +99,9 @@ def OpenExhaustive (G : Intermediate.GlobalEnv) : Prop :=
   Intermediate.lookup x G = some (Intermediate.Entry.openm x cls ⟨na, Ks1, nb, Ks2, nc, Ts, R⟩) ->
   Intermediate.Query G .opn q Ts ->
   ∃ (i : Nat), ∃ n cls_name k1 k2 k3 Ks1 Ks2 tys fds scs mths, G[i]? = some (.instDecl ⟨n, cls_name, k1, k2, k3, Ks1, Ks2, tys, fds, scs, mths⟩)
-    ∧ ∃ (j : Nat), ((∃ b p, fds[j]? = some ⟨x, nc, p, b⟩ ∧ Core.Query.Match q p)
-                   ∨ (∃ b p, scs[j]? = some ⟨x, nc, p, b⟩ ∧ Core.Query.Match q p)
-                   ∨ (∃ b p, mths[j]? = some ⟨x, nc, p, b⟩ ∧ Core.Query.Match q p))
+    ∧ ((∃ (j : Nat), ∃ b p, fds[j]? = some ⟨x, nc, p, b⟩ ∧ Core.Query.Match q p)
+       ∨ (∃ (j : Nat), ∃ b p, scs[j]? = some ⟨x, nc, p, b⟩ ∧ Core.Query.Match q p)
+       ∨ (∃ (j : Nat), ∃ b p, mths[j]? = some ⟨x, nc, p, b⟩ ∧ Core.Query.Match q p))
 
 notation:175 "Ω " G:175 => OpenExhaustive G
 
